Break up and rename some files

src/Eval.v
@@ -1,429 +1,138 @@
-Require Import
-  Coq.Unicode.Utf8
-  Coq.Lists.List
-  Coq.Relations.Relation_Definitions
-  Coq.Classes.RelationClasses
-  Coq.Classes.Morphisms
+Require Export
   Ty
   Exp
   Sub
-  Sem.
+  Sem
+  Eval
+  Norm.
 
 From Equations Require Import Equations.
 
-Section Eval.
-
 Generalizable All Variables.
 
+Section Eval.
+
 Import ListNotations.
-
-Context {A : Type}.
-Context `{S : HostExprsSem A}.
-
-Reserved Notation " t '--->' t' " (at level 40).
-
-(************************************************************************
- * Small-step operational semantics
- *)
-
-Inductive Step : ∀ {Γ τ}, Exp Γ τ → Exp Γ τ → Prop :=
-  | ST_Seq Γ τ τ' (e1 : Exp Γ τ') (e2 : Exp Γ τ) :
-    Seq e1 e2 ---> e2
-
-  | ST_Host Γ τ (h : HostExp τ) :
-    HostedExp h ---> projT1 (Reduce (Γ:=Γ) h)
-
-  | ST_IfTrue Γ τ (t e : Exp Γ τ) :
-    If ETrue t e ---> t
-  | ST_IfFalse Γ τ (t e : Exp Γ τ) :
-    If EFalse t e ---> e
-  | ST_If Γ b b' τ (t e : Exp Γ τ) :
-    b ---> b' →
-    If b t e ---> If b' t e
-
-  | ST_Pair1 Γ τ1 τ2 (x x' : Exp Γ τ1) (y : Exp Γ τ2) :
-    x ---> x' →
-    Pair x y ---> Pair x' y
-  | ST_Pair2 Γ τ1 τ2 (x : Exp Γ τ1) (y y' : Exp Γ τ2) :
-    ValueP x →
-    y ---> y' →
-    Pair x y ---> Pair x y'
-
-  | ST_Fst1 Γ τ1 τ2 (p p' : Exp Γ (TyPair τ1 τ2)) :
-    p ---> p' →
-    Fst p ---> Fst p'
-  | ST_FstPair Γ τ1 τ2 (v1 : Exp Γ τ1) (v2 : Exp Γ τ2) :
-    ValueP v1 →
-    ValueP v2 →
-    Fst (Pair v1 v2) ---> v1
-
-  | ST_Snd1 Γ τ1 τ2 (p p' : Exp Γ (TyPair τ1 τ2)) :
-    p ---> p' →
-    Snd p ---> Snd p'
-  | ST_SndPair Γ τ1 τ2 (v1 : Exp Γ τ1) (v2 : Exp Γ τ2) :
-    ValueP v1 →
-    ValueP v2 →
-    Snd (Pair v1 v2) ---> v2
-
-  | ST_Cons1 Γ τ (x : Exp Γ τ) x' (xs : Exp Γ (TyList τ)) :
-    x ---> x' →
-    Cons x xs ---> Cons x' xs
-  | ST_Cons2 Γ τ (x : Exp Γ τ) (xs : Exp Γ (TyList τ)) xs' :
-    ValueP x →
-    xs ---> xs' →
-    Cons x xs ---> Cons x xs'
-
-  | ST_Car1 Γ τ (d d' : Exp Γ τ) (l : Exp Γ (TyList τ)) :
-    d ---> d' →
-    Car d l ---> Car d' l
-  | ST_Car2 Γ τ (d : Exp Γ τ) (l l' : Exp Γ (TyList τ)) :
-    ValueP d →
-    l ---> l' →
-    Car d l ---> Car d l'
-  | ST_CarNil Γ τ (d : Exp Γ τ) :
-    ValueP d →
-    Car d Nil ---> d
-  | ST_CarCons Γ τ (d x : Exp Γ τ) (xs : Exp Γ (TyList τ)) :
-    ValueP d →
-    ValueP x →
-    ValueP xs →
-    Car d (Cons x xs) ---> x
-
-  | ST_Cdr1 Γ τ (l l' : Exp Γ (TyList τ)) :
-    l ---> l' →
-    Cdr l ---> Cdr l'
-  | ST_CdrNil Γ τ :
-    Cdr (Nil (Γ:=Γ) (τ:=τ)) ---> Nil
-  | ST_CdrCons Γ τ (x : Exp Γ τ) (xs : Exp Γ (TyList τ)) :
-    ValueP x →
-    ValueP xs →
-    Cdr (Cons x xs) ---> xs
-
-  | ST_AppHost Γ dom cod (f : HostExp (dom ⟶ cod)) (v : Exp Γ dom) :
-    ∀ H : ValueP v,
-    APP (HostedFun f) v ---> CallHost f v H
-
-  | ST_AppAbs Γ dom cod (e : Exp (dom :: Γ) cod) (v : Exp Γ dom) :
-    ValueP v →
-    APP (LAM e) v ---> SubExp {|| v ||} e
-
-  | ST_App1 Γ dom cod (e1 : Exp Γ (dom ⟶ cod)) e1' (e2 : Exp Γ dom) :
-    e1 ---> e1' →
-    APP e1 e2 ---> APP e1' e2
-
-  | ST_App2 Γ dom cod (v1 : Exp Γ (dom ⟶ cod)) (e2 : Exp Γ dom) e2' :
-    ValueP v1 →
-    e2 ---> e2' →
-    APP v1 e2 ---> APP v1 e2'
-
-  where " t '--->' t' " := (Step t t').
-
-Derive Signature for Step.
-
-Inductive multi `(R : relation X) : relation X :=
-  | multi_refl (x : X) : multi R x x
-  | multi_step (x y z : X) :
-      R x y → multi R y z → multi R x z.
-
-Derive Signature for multi.
-
-Theorem multi_R `(R : relation X) (x y : X) :
-  R x y → multi R x y.
-Proof.
-  intros.
-  eapply multi_step; eauto.
-  now constructor.
-Qed.
-
-Theorem multi_trans `(R : relation X) (x y z : X) :
-  multi R x y →
-  multi R y z →
-  multi R x z.
-Proof.
-  intros.
-  induction H; auto.
-  now eapply multi_step; eauto.
-Qed.
-
-#[export]
-Program Instance multi_PreOrder `(R : relation X) :
-  PreOrder (multi R).
-Next Obligation. now constructor. Qed.
-Next Obligation. now eapply multi_trans; eauto. Qed.
-
-#[export]
-Program Instance Step_respects {Γ τ} :
-  Proper (Step --> Step ==> impl) (multi (Step (Γ:=Γ) (τ:=τ))).
-Next Obligation.
-  econstructor; eauto.
-  generalize dependent y0.
-  generalize dependent y.
-  induction H1; intros; eauto.
-  - now repeat econstructor; eauto.
-  - unfold flip in *.
-    now econstructor; eauto.
-Qed.
-
-End Eval.
-
-Notation " t '--->' t' " := (Step t t') (at level 40).
-Notation " t '--->*' t' " := (multi Step t t') (at level 40).
-
-Class HostLang (A : Type) : Type := {
-  has_host_exprs_sem :> HostExprsSem A;
-
-
-  CallHost_sound {Γ dom cod} (f : HostExp (dom ⟶ cod))
-                 (v : Exp Γ dom) (H : ValueP v) se :
-    HostExpSem f (SemExp v se) = SemExp (CallHost f v H) se;
-
-  CallHost_irr {Γ dom cod} (f : HostExp (dom ⟶ cod))
-               (v : Exp Γ dom) (H : ValueP v) :
-    ¬ (CallHost f v H = APP (HostedFun f) v);
-
-  CallHost_preserves_renaming {Γ Γ' dom cod} (f : HostExp (dom ⟶ cod))
-               (v : Exp Γ dom) (H : ValueP v) (σ : Ren Γ' Γ) :
-    APP (HostedFun f) (RenExp σ v) ---> RenExp σ (CallHost f v H);
-
-  CallHost_preserves_substitution {Γ Γ' dom cod} (f : HostExp (dom ⟶ cod))
-               (v : Exp Γ dom) (H : ValueP v) (σ : Sub Γ' Γ) :
-    APP (HostedFun f) (SubExp σ v) ---> SubExp σ (CallHost f v H);
-
-
-  Reduce_sound {Γ τ} (h : HostExp τ) se :
-    HostExpSem h = SemExp (projT1 (Reduce (Γ:=Γ) h)) se;
-
-  Reduce_irr {Γ τ} (h : HostExp τ) :
-    ¬ (projT1 (Reduce (Γ:=Γ) h) = HostedExp h);
-
-  Reduce_preserves_renaming {Γ Γ' τ} (h : HostExp τ) (σ : Ren Γ Γ') :
-    RenExp σ (HostedExp h) ---> RenExp σ (projT1 (Reduce h));
-
-  Reduce_preserves_substitution {Γ Γ' τ} (h : HostExp τ) (σ : Sub Γ Γ') :
-    SubExp σ (HostedExp h) ---> SubExp σ (projT1 (Reduce h));
-}.
-
-Section Sound.
 
 Context {A : Type}.
 Context `{L : HostLang A}.
 
-Theorem Step_sound {Γ τ} (e : Exp Γ τ) v :
-  e ---> v → SemExp e = SemExp v.
+Inductive Kont : Ty → Ty → Type :=
+  | MT {a}   : Kont a a
+  | FN {a b} : (Value a → Σ b) → Kont a b
+
+with Σ : Ty → Type :=
+  | MkΣ {Γ    : Env}
+        {τ    : Ty}
+        {r    : Ty}
+        (exp  : Exp Γ r)
+        (env  : ValEnv Γ)
+        (knt  : Kont r τ) : Σ τ.
+
+Derive Signature NoConfusion Subterm for Kont.
+Derive Signature NoConfusion NoConfusionHom Subterm for Σ.
+
+Equations with_closure `(a : Exp Γ dom) `(ρ : ValEnv Γ)
+          `(κ : Kont cod τ) `(f : Value (dom ⟶ cod)) : Σ τ :=
+  with_closure a ρ κ (ClosureExp (Lambda e)) :=
+    MkΣ a ρ (FN (λ v, MkΣ e (Val v Empty) κ));
+  with_closure a ρ κ (ClosureExp (Func f)) :=
+    MkΣ a ρ (FN (λ v, let '(existT _ x H) := valueToExp v in
+                      MkΣ (CallHost f x H) Empty κ)).
+
+Equations IfBody `(v : Value TyBool) {Γ τ} (t e : Exp Γ τ) : Exp Γ τ :=
+  IfBody VTrue  t _ := t;
+  IfBody VFalse _ e := e.
+
+Equations VFst `(v : Value (TyPair τ1 τ2)) : Value τ1 :=
+  VFst (VPair x _) := x.
+
+Equations VSnd `(v : Value (TyPair τ1 τ2)) : Value τ2 :=
+  VSnd (VPair _ y) := y.
+
+Equations VCar `(v : Value (TyList r)) {Γ} (d : Exp Γ r) (ρ : ValEnv Γ)
+          `(κ : Kont r τ) : Σ τ :=
+  VCar VNil        d ρ κ := MkΣ d ρ κ;
+  VCar (VCons x _) _ _ κ := MkΣ (projT1 (valueToExp x)) Empty κ.
+
+Equations VCdr `(v : Value (TyList r)) {Γ} (ρ : ValEnv Γ)
+          `(κ : Kont (TyList r) τ) : Σ τ :=
+  VCdr VNil         ρ κ := MkΣ Nil ρ κ;
+  VCdr (VCons _ xs) _ κ := MkΣ (projT1 (valueToExp xs)) Empty κ.
+
+Equations step {τ : Ty} (s : Σ τ) : Σ τ :=
+  (* Constants *)
+  step (MkΣ (r:=TyHost _)   (HostedVal x) ρ (FN f)) := f (HostValue x);
+  step (MkΣ (r:=dom ⟶ cod) (HostedFun x) ρ (FN f)) := f (ClosureExp (Func x));
+  step (MkΣ (HostedExp x) ρ κ) := MkΣ (projT1 (Reduce x)) ρ κ;
+
+  step (MkΣ EUnit  _ (FN f)) := f VUnit;
+  step (MkΣ ETrue  _ (FN f)) := f VTrue;
+  step (MkΣ EFalse _ (FN f)) := f VFalse;
+
+  step (MkΣ (If b th el) ρ κ) :=
+    MkΣ b ρ (FN (λ v, MkΣ (IfBody v th el) ρ κ));
+
+  step (MkΣ (Pair x y) ρ (FN f)) :=
+    MkΣ x ρ (FN (λ v1, MkΣ y ρ (FN (λ v2, f (VPair v1 v2)))));
+  step (MkΣ (Fst p) ρ κ) :=
+    MkΣ p ρ (FN (λ p, MkΣ (projT1 (valueToExp (VFst p))) Empty κ));
+  step (MkΣ (Snd p) ρ κ) :=
+    MkΣ p ρ (FN (λ p, MkΣ (projT1 (valueToExp (VSnd p))) Empty κ));
+
+  step (MkΣ Nil _ (FN f)) := f VNil;
+  step (MkΣ (Cons x xs) ρ (FN f)) :=
+    MkΣ x ρ (FN (λ v1, MkΣ xs ρ (FN (λ v2, f (VCons v1 v2)))));
+  step (MkΣ (Car d xs) ρ κ) :=
+    MkΣ xs ρ (FN (λ l, VCar l d ρ κ));
+  step (MkΣ (Cdr xs) ρ κ) :=
+    MkΣ xs ρ (FN (λ l, VCdr l ρ κ));
+
+  (* A sequence just evaluates the second, for now *)
+  step (MkΣ (Seq e1 e2) ρ κ) := MkΣ e2 ρ κ;
+
+  (* A variable might lookup a lambda, in which case continue evaluating down
+     that vein; otherwise, if no continuation, this is as far as we can go. *)
+  step (MkΣ (VAR v) ρ κ) with get_value ρ v := {
+    | x with κ := {
+        | MT   => MkΣ (projT1 (valueToExp x)) Empty κ
+        | FN f => f x
+      }
+  };
+
+  (* If a lambda is passed, call it with the continuation *)
+  step (MkΣ (LAM e) ρ (FN f)) := f (ClosureExp (Lambda (vsubst e ρ)));
+
+  (* Application evaluates the lambda and then the argument *)
+  step (MkΣ (APP e1 e2) ρ κ) := MkΣ e1 ρ (FN (with_closure e2 ρ κ));
+
+  step (MkΣ e ρ MT) := MkΣ e ρ MT.
+
+Equations loop (gas : nat) {τ : Ty} (s : Σ τ) : Σ τ :=
+  loop O s := s;
+  loop (S gas') s := loop gas' (step s).
+
+(* Inject the expression into a [Σ] whose final continuation will receive the
+   results of the evaluation. Therefore, the resulting [env] will be a
+   singleton list containing that value. *)
+Definition inject {τ : Ty} (e : Exp [] τ) : Σ τ := MkΣ e Empty MT.
+
+Definition run (gas : nat) {τ : Ty} (e : Exp [] τ) : Σ τ := loop gas (inject e).
+
+Ltac ceksimp :=
+  repeat (simp loop;
+          simp step;
+          simp IfBody;
+          simp VFst;
+          simp VSnd;
+          simpl).
+
+Ltac is_step := ceksimp; firstorder eauto.
+
+Theorem cek_sound τ (e e' : Exp [] τ) :
+  e --->* e' → ValueP e' →      (* evaluation halts at e' *)
+  ∃ gas, loop gas (inject e) = MkΣ e' Empty MT.
 Proof.
-  intros.
-  dependent induction H; simpl; auto;
-  extensionality se;
-  try now rewrite IHStep.
-  - now erewrite Reduce_sound; eauto.
-  - now apply CallHost_sound.
-  - rewrite <- SemExp_SubSem.
-    f_equal; simpl.
-    simp SubSem.
-    now rewrite SubSem_idSub.
-Qed.
+Abort.
 
-Lemma If_loop_true {Γ τ} b {x : Exp Γ τ} {y : Exp Γ τ} :
-  ¬ (If b x y = x).
-Proof.
-  induction x; intro; inv H.
-  now eapply IHx2; eauto.
-Qed.
-
-Lemma If_loop_false {Γ τ} b {x : Exp Γ τ} {y : Exp Γ τ} :
-  ¬ (If b x y = y).
-Proof.
-  induction y; intro; inv H.
-  now eapply IHy3; eauto.
-Qed.
-
-Lemma Seq_loop {Γ τ ty} {x : Exp Γ ty} {y : Exp Γ τ} :
-  ¬ (Seq x y = y).
-Proof.
-  induction y; intro; inv H.
-  now eapply IHy2; eauto.
-Qed.
-
-Lemma App_Lam_loop {Γ τ ty} {v : Exp Γ ty} {e : Exp (ty :: Γ) τ} :
-  ¬ (SubExp {||v||} e = APP (LAM e) v).
-Proof.
-  dependent induction e; repeat intro; inv H.
-  - dependent induction v0; simp consSub in *.
-    + simp SubVar in H1.
-      now induction v; inv H1; intuition.
-    + simp SubVar in H1.
-      rewrite SubVar_idSub in H1.
-      now induction v0; inv H1; intuition.
-  - admit.
-Admitted.
-
-(* A term never reduces to itself. *)
-#[export]
-Program Instance Step_Irreflexive {Γ τ} :
-  Irreflexive (Step (Γ:=Γ) (τ:=τ)).
-Next Obligation.
-  dependent induction x; try solve [ now inv H ].
-  - inv H.
-    + now apply Reduce_irr in H4.
-  - inv H.
-    + now eapply If_loop_true; eauto.
-    + now eapply If_loop_false; eauto.
-    + now firstorder.
-  - inv H.
-    now eapply Seq_loop; eauto.
-  - inv H.
-    + now eapply CallHost_irr; eauto.
-    + now eapply App_Lam_loop; eauto.
-    + now eapply IHx1; eauto.
-    + now eapply IHx2; eauto.
-Qed.
-
-#[export]
-Program Instance RenExp_Step {Γ Γ' τ} (σ : Ren Γ' Γ) :
-  Proper (Step (Γ:=Γ) (τ:=τ) ==> Step) (RenExp σ).
-Next Obligation.
-  intros.
-  induction H; simpl;
-  try solve [ now constructor; intuition idtac
-            | now constructor; intuition; apply RenExp_ValueP ].
-  - now apply Reduce_preserves_renaming.
-  - now apply CallHost_preserves_renaming.
-  - rewrite <- SubExp_ScR.
-    simp ScR.
-    rewrite <- RcS_idSub.
-    pose proof (SubExp_RcS (Keep σ) (Push (RenExp σ v) idSub) e).
-    simp RcS in H.
-    rewrite H.
-    constructor.
-    now apply RenExp_ValueP.
-Qed.
-
-#[export]
-Program Instance SubExp_Step {Γ Γ' τ} (σ : Sub Γ' Γ) :
-  Proper (Step (Γ:=Γ) (τ:=τ) ==> Step) (SubExp σ).
-Next Obligation.
-  intros.
-  induction H; simpl;
-  try solve [ now constructor; intuition idtac
-            | now constructor; intuition; apply SubExp_ValueP ].
-  - now apply Reduce_preserves_substitution.
-  - now apply CallHost_preserves_substitution.
-  - rewrite <- SubExp_ScS.
-    simpl ScS.
-    rewrite ScS_idSub_left.
-    pose proof (SubExp_ScS (Keepₛ σ) (Push (SubExp σ v) idSub) e).
-    simpl in H.
-    simp SubVar in H.
-    unfold Dropₛ in H.
-    rewrite ScS_ScR in H.
-    rewrite RcS_skip1 in H.
-    rewrite ScS_idSub_right in H.
-    rewrite H.
-    constructor.
-    now apply SubExp_ValueP.
-Qed.
-
-Corollary Step_productive {Γ τ} {x x' : Exp Γ τ} : x ---> x' → x ≠ x'.
-Proof.
-  repeat intro; subst.
-  now eapply Step_Irreflexive; eauto.
-Qed.
-
-Import ListNotations.
-
-Theorem strong_progress {τ} (e : Exp [] τ) :
-  ValueP e + { e' | e ---> e' }.
-Proof.
-  dependent induction e; reduce.
-  - destruct τ;
-    right; now exists (projT1 (Reduce h)); constructor.
-  - now left; constructor.
-  - now left; constructor.
-  - now left; constructor.
-  - now left; constructor.
-  - now left; constructor.
-  - right.
-    destruct IHe1; reduce.
-    + inv v.
-      * now exists e2; constructor.
-      * now exists e3; constructor.
-    + reduce.
-      now exists (If x e2 e3); constructor.
-  - destruct IHe1; reduce.
-    + destruct IHe2; reduce.
-      * left.
-        now constructor.
-      * right; reduce.
-        now exists (Pair e1 x); constructor.
-    + destruct IHe2; reduce.
-      * right; reduce.
-        now exists (Pair x e2); constructor.
-      * right; reduce.
-        now exists (Pair x e2); constructor.
-  - destruct IHe; reduce.
-    + right.
-      inv v; reduce.
-      * now exists x; constructor.
-    + right; reduce.
-      now exists (Fst x); constructor.
-  - destruct IHe; reduce.
-    + right.
-      inv v.
-      * now exists y; constructor.
-    + right; reduce.
-      now exists (Snd x); constructor.
-  - now left; constructor.
-  - destruct IHe1.
-    + destruct IHe2.
-      * now left; constructor.
-      * right; reduce.
-        now exists (Cons e1 x); constructor.
-    + destruct IHe2.
-      * right; reduce.
-        now exists (Cons x e2); constructor.
-      * right; reduce.
-        now exists (Cons x0 e2); constructor.
-  - destruct IHe1.
-    + destruct IHe2.
-      * right.
-        inv v0.
-        ** now eexists; constructor.
-        ** now eexists; constructor.
-      * right; reduce.
-        now exists (Car e1 x); constructor.
-    + destruct IHe2.
-      * right; reduce.
-        now exists (Car x e2); constructor.
-      * right; reduce.
-        now exists (Car x0 e2); constructor.
-  - destruct IHe.
-    + right.
-      inv v; now eexists; constructor.
-    + right; reduce.
-      now exists (Cdr x); constructor.
-  - right.
-    now exists e2; constructor.
-  - now inversion v.
-  - left.
-    now constructor.
-  - right.
-    destruct IHe1.
-    + destruct IHe2.
-      * dependent elimination e1; inv v.
-        ** now exists (CallHost h1 e2 v0); constructor.
-        ** now eexists (SubExp {|| e2 ||} _); constructor.
-      * dependent elimination e1; inv v.
-        ** exists (APP (HostedFun h1) x); constructor; auto.
-           now constructor.
-        ** eexists (APP (LAM _) x); constructor; eauto.
-           now constructor.
-    + reduce.
-      destruct IHe2.
-      * exists (APP x e2).
-        now constructor.
-      * reduce.
-        exists (APP x e2).
-        now constructor.
-Qed.
-
-End Sound.
+End Eval.
