src/Multi.v
@@ -1,0 +1,291 @@
+Require Export
+  Coq.Unicode.Utf8
+  Coq.Lists.List
+  Coq.Relations.Relation_Definitions
+  Coq.Classes.RelationClasses
+  Coq.Classes.Morphisms
+  Ty
+  Exp
+  Sub
+  Sem
+  Step.
+
+From Equations Require Import Equations.
+
+Section Multi.
+
+Generalizable All Variables.
+
+Import ListNotations.
+
+Context {A : Type}.
+Context `{S : HostExprsSem A}.
+
+Inductive multi `(R : relation X) : relation X :=
+  | multi_refl (x : X) : multi R x x
+  | multi_step (x y z : X) :
+      R x y → multi R y z → multi R x z.
+
+Derive Signature for multi.
+
+Theorem multi_R `(R : relation X) (x y : X) :
+  R x y → multi R x y.
+Proof.
+  intros.
+  eapply multi_step; eauto.
+  now constructor.
+Qed.
+
+Theorem multi_trans `(R : relation X) (x y z : X) :
+  multi R x y →
+  multi R y z →
+  multi R x z.
+Proof.
+  intros.
+  induction H; auto.
+  now eapply multi_step; eauto.
+Qed.
+
+#[export]
+Program Instance multi_PreOrder `(R : relation X) :
+  PreOrder (multi R).
+Next Obligation. now constructor. Qed.
+Next Obligation. now eapply multi_trans; eauto. Qed.
+
+#[export]
+Program Instance multi_respects_Step {Γ τ} :
+  Proper (Step --> Step ==> impl) (multi (Step (Γ:=Γ) (τ:=τ))).
+Next Obligation.
+  econstructor; eauto.
+  generalize dependent y0.
+  generalize dependent y.
+  induction H1; intros; eauto.
+  - now repeat econstructor; eauto.
+  - unfold flip in *.
+    now econstructor; eauto.
+Qed.
+
+Notation " t '--->*' t' " := (multi Step t t') (at level 40).
+
+Lemma multistep_Seq {Γ τ} {e1 : Γ ⊢ τ} {τ'} {e2 : Γ ⊢ τ'} :
+  Seq e1 e2 --->* e2.
+Proof.
+  intros.
+  eapply multi_step; eauto.
+  - now constructor.
+  - now apply multi_refl.
+Qed.
+
+Ltac simpl_multistep :=
+  intros;
+  match goal with
+  | [ H : _ --->* _ |- _ ] => induction H
+  end;
+  [ now apply multi_refl
+  | eapply multi_step; eauto;
+    now constructor ].
+
+Lemma multistep_If {Γ} {e1 e1' : Γ ⊢ TyBool} {τ} {e2 e3 : Γ ⊢ τ} :
+  (e1 --->* e1') → If e1 e2 e3 --->* If e1' e2 e3.
+Proof. now simpl_multistep. Qed.
+
+Lemma multistep_Pair1 {Γ τ1 τ2} {e1 e1' : Γ ⊢ τ1} {e2 : Γ ⊢ τ2} :
+  (e1 --->* e1') → Pair e1 e2 --->* Pair e1' e2.
+Proof. now simpl_multistep. Qed.
+
+Lemma multistep_Pair2 {Γ τ1 τ2} {e1 : Γ ⊢ τ1} {e2 e2' : Γ ⊢ τ2} :
+  ValueP e1 → (e2 --->* e2') → Pair e1 e2 --->* Pair e1 e2'.
+Proof. now simpl_multistep. Qed.
+
+Lemma multistep_Pair {Γ τ1 τ2} {e1 e1' : Γ ⊢ τ1} {e2 e2' : Γ ⊢ τ2} :
+  ValueP e1' →
+  (e1 --->* e1') → (e2 --->* e2') → Pair e1 e2 --->* Pair e1' e2'.
+Proof.
+  intros.
+  induction H; simpl; intros; reduce.
+  - now apply multistep_Pair2; auto.
+  - rewrite <- IHmulti; auto.
+    apply multistep_Pair1; auto.
+    now econstructor; eauto.
+Qed.
+
+Lemma multistep_Fst1 {Γ τ1 τ2} {p p' : Γ ⊢ (τ1 × τ2)} :
+  (p --->* p') → Fst p --->* Fst p'.
+Proof. now simpl_multistep. Qed.
+
+Lemma multistep_FstPair {Γ τ1 τ2} {e1 e1' : Γ ⊢ τ1} {e2 e2' : Γ ⊢ τ2} :
+  ValueP e1' → (e1 --->* e1') →
+  ValueP e2' → (e2 --->* e2') → Fst (Pair e1 e2) --->* e1'.
+Proof.
+  intros.
+  induction H; intros.
+  - induction H0; intros.
+    + apply multi_R.
+      now constructor.
+    + rewrite <- IHmulti at 2; auto.
+      apply multistep_Fst1.
+      apply multistep_Pair; eauto.
+      constructor.
+      now apply multi_R.
+  - rewrite <- IHmulti; auto.
+    apply multistep_Fst1; auto.
+    apply multistep_Pair1; auto.
+    now apply multi_R.
+Qed.
+
+Lemma multistep_Snd1 {Γ τ1 τ2} {p p' : Γ ⊢ (τ1 × τ2)} :
+  (p --->* p') → Snd p --->* Snd p'.
+Proof. now simpl_multistep. Qed.
+
+Lemma multistep_SndPair {Γ τ1 τ2} {e1 e1' : Γ ⊢ τ1} {e2 e2' : Γ ⊢ τ2} :
+  ValueP e1' → (e1 --->* e1') →
+  ValueP e2' → (e2 --->* e2') → Snd (Pair e1 e2) --->* e2'.
+Proof.
+  intros.
+  induction H; intros.
+  - induction H0; intros.
+    + apply multi_R.
+      now constructor.
+    + rewrite <- IHmulti; auto.
+      apply multistep_Snd1.
+      apply multistep_Pair; eauto.
+      constructor.
+      now apply multi_R.
+  - rewrite <- IHmulti; auto.
+    apply multistep_Snd1; auto.
+    apply multistep_Pair1; auto.
+    now apply multi_R.
+Qed.
+
+Lemma multistep_Cons1 {Γ τ} {x x' : Γ ⊢ τ} {xs : Γ ⊢ (TyList τ)} :
+  (x --->* x') → Cons x xs --->* Cons x' xs.
+Proof. now simpl_multistep. Qed.
+
+Lemma multistep_Cons2 {Γ τ} {x : Γ ⊢ τ} {xs xs' : Γ ⊢ (TyList τ)} :
+  ValueP x → (xs --->* xs') → Cons x xs --->* Cons x xs'.
+Proof. now simpl_multistep. Qed.
+
+Lemma multistep_Cons {Γ τ} {e1 e1' : Γ ⊢ τ} {e2 e2' : Γ ⊢ (TyList τ)} :
+  ValueP e1' →
+  (e1 --->* e1') → (e2 --->* e2') → Cons e1 e2 --->* Cons e1' e2'.
+Proof.
+  intros.
+  induction H; intros.
+  - now apply multistep_Cons2; auto.
+  - rewrite <- IHmulti; auto.
+    apply multistep_Cons1; auto.
+    now econstructor; eauto.
+Qed.
+
+Lemma multistep_Car1 {Γ τ} {d d' : Γ ⊢ τ} {xs : Γ ⊢ (TyList τ)} :
+  (d --->* d') → Car d xs --->* Car d' xs.
+Proof. now simpl_multistep. Qed.
+
+Lemma multistep_Car2 {Γ τ} {d : Γ ⊢ τ} {xs xs' : Γ ⊢ (TyList τ)} :
+  ValueP d → (xs --->* xs') → Car d xs --->* Car d xs'.
+Proof. now simpl_multistep. Qed.
+
+Lemma multistep_Car {Γ τ} {d d' : Γ ⊢ τ} {xs xs' : Γ ⊢ (TyList τ)} :
+  ValueP d' →
+  (d --->* d') → (xs --->* xs') → Car d xs --->* Car d' xs'.
+Proof.
+  intros.
+  induction H; intros.
+  - now apply multistep_Car2.
+  - rewrite <- IHmulti; eauto.
+    apply multistep_Car1; auto.
+    now econstructor; eauto.
+Qed.
+
+Lemma multistep_CarNil {Γ τ} {d d' : Γ ⊢ τ} {xs : Γ ⊢ (TyList τ)} :
+  ValueP d' → (d --->* d') →
+  (xs --->* Nil) → Car d xs --->* d'.
+Proof.
+  intros.
+  dependent induction H.
+  - erewrite multistep_Car2; eauto.
+    apply multi_R.
+    now constructor.
+  - rewrite <- IHmulti; eauto.
+    apply multistep_Car1.
+    now apply multi_R.
+Qed.
+
+Lemma multistep_CarCons {Γ τ} {d e1 : Γ ⊢ τ} {e2 xs : Γ ⊢ (TyList τ)} :
+  ValueP d → ValueP e1 → ValueP e2 →
+  (xs --->* Cons e1 e2) → Car d xs --->* e1.
+Proof.
+  intros.
+  dependent induction H.
+  - erewrite multistep_Car2; eauto.
+    + apply multi_R.
+      now constructor; eauto.
+    + now constructor; eauto.
+  - specialize (IHmulti _ _ _ d _ _ _ X X0 X1
+                        eq_refl JMeq_refl JMeq_refl JMeq_refl).
+    rewrite <- IHmulti; auto.
+    apply multistep_Car2; auto.
+    now apply multi_R.
+Fail Qed.
+Admitted.
+
+Lemma multistep_Cdr1 {Γ τ} {xs xs' : Γ ⊢ (TyList τ)} :
+  (xs --->* xs') → Cdr xs --->* Cdr xs'.
+Proof. now simpl_multistep. Qed.
+
+Lemma multistep_CdrNil {Γ τ} {xs : Γ ⊢ (TyList τ)} :
+  (xs --->* Nil) → Cdr xs --->* Nil.
+Proof.
+  intros.
+  dependent induction H.
+  - apply multi_R.
+    now constructor.
+  - rewrite <- IHmulti; eauto.
+    apply multi_R.
+    now constructor.
+Qed.
+
+Lemma multistep_CdrCons {Γ τ} {e1 : Γ ⊢ τ} {e2 xs : Γ ⊢ (TyList τ)} :
+  ValueP e1 → ValueP e2 →
+  (xs --->* Cons e1 e2) → Cdr xs --->* e2.
+Proof.
+  intros.
+  dependent induction H.
+  - apply multi_R.
+    now constructor.
+  - specialize (IHmulti _ _ _ _ _ y X X0
+                        eq_refl JMeq_refl JMeq_refl JMeq_refl).
+    rewrite <- IHmulti.
+    apply multistep_Cdr1.
+    now apply multi_R.
+Fail Qed.
+Admitted.
+
+(*
+Lemma multistep_CdrCons {Γ τ} {e1 e1' : Γ ⊢ τ} {e2 e2' : Γ ⊢ (TyList τ)} :
+  ValueP e1' → (e1 --->* e1') →
+  ValueP e2' → (e2 --->* e2') → Cdr (Cons e1 e2) --->* e2'.
+Proof.
+  intros.
+  induction H; intros.
+  - induction H0; intros.
+    + apply multi_R.
+      now constructor.
+    + rewrite <- IHmulti; auto.
+      apply multistep_Cdr1.
+      apply multistep_Cons2; eauto.
+      now apply multi_R.
+  - rewrite <- IHmulti; auto.
+    apply multistep_Cdr1; auto.
+    apply multistep_Cons1; auto.
+    now apply multi_R.
+Qed.
+*)
+
+Lemma multistep_App2 {Γ dom cod} {e e' : Γ ⊢ dom} {v : Γ ⊢ (dom ⟶ cod)} :
+  ValueP v → (e --->* e') → APP v e --->* APP v e'.
+Proof. now simpl_multistep. Qed.
+
+End Multi.
+
+Notation " t '--->*' t' " := (multi Step t t') (at level 40).
