src/Step.v
@@ -1,0 +1,383 @@
+Require Import
+  Coq.Unicode.Utf8
+  Coq.Lists.List
+  Coq.Classes.RelationClasses
+  Coq.Classes.Morphisms
+  Ty
+  Exp
+  Sub
+  Sem.
+
+From Equations Require Import Equations.
+
+Section Step.
+
+Generalizable All Variables.
+
+Import ListNotations.
+
+Context {A : Type}.
+Context `{S : HostExprsSem A}.
+
+Reserved Notation " t '--->' t' " (at level 40).
+
+(************************************************************************
+ * Small-step operational semantics
+ *)
+
+Inductive Step : ∀ {Γ τ}, Exp Γ τ → Exp Γ τ → Prop :=
+  | ST_Seq Γ τ τ' (e1 : Exp Γ τ') (e2 : Exp Γ τ) :
+    Seq e1 e2 ---> e2
+
+  | ST_Host Γ τ (h : HostExp τ) :
+    HostedExp h ---> projT1 (Reduce (Γ:=Γ) h)
+
+  | ST_IfTrue Γ τ (t e : Exp Γ τ) :
+    If ETrue t e ---> t
+  | ST_IfFalse Γ τ (t e : Exp Γ τ) :
+    If EFalse t e ---> e
+  | ST_If Γ b b' τ (t e : Exp Γ τ) :
+    b ---> b' →
+    If b t e ---> If b' t e
+
+  | ST_Pair1 Γ τ1 τ2 (x x' : Exp Γ τ1) (y : Exp Γ τ2) :
+    x ---> x' →
+    Pair x y ---> Pair x' y
+  | ST_Pair2 Γ τ1 τ2 (x : Exp Γ τ1) (y y' : Exp Γ τ2) :
+    ValueP x →
+    y ---> y' →
+    Pair x y ---> Pair x y'
+
+  | ST_Fst1 Γ τ1 τ2 (p p' : Exp Γ (TyPair τ1 τ2)) :
+    p ---> p' →
+    Fst p ---> Fst p'
+  | ST_FstPair Γ τ1 τ2 (v1 : Exp Γ τ1) (v2 : Exp Γ τ2) :
+    ValueP v1 →
+    ValueP v2 →
+    Fst (Pair v1 v2) ---> v1
+
+  | ST_Snd1 Γ τ1 τ2 (p p' : Exp Γ (TyPair τ1 τ2)) :
+    p ---> p' →
+    Snd p ---> Snd p'
+  | ST_SndPair Γ τ1 τ2 (v1 : Exp Γ τ1) (v2 : Exp Γ τ2) :
+    ValueP v1 →
+    ValueP v2 →
+    Snd (Pair v1 v2) ---> v2
+
+  | ST_Cons1 Γ τ (x : Exp Γ τ) x' (xs : Exp Γ (TyList τ)) :
+    x ---> x' →
+    Cons x xs ---> Cons x' xs
+  | ST_Cons2 Γ τ (x : Exp Γ τ) (xs : Exp Γ (TyList τ)) xs' :
+    ValueP x →
+    xs ---> xs' →
+    Cons x xs ---> Cons x xs'
+
+  | ST_Car1 Γ τ (d d' : Exp Γ τ) (l : Exp Γ (TyList τ)) :
+    d ---> d' →
+    Car d l ---> Car d' l
+  | ST_Car2 Γ τ (d : Exp Γ τ) (l l' : Exp Γ (TyList τ)) :
+    ValueP d →
+    l ---> l' →
+    Car d l ---> Car d l'
+  | ST_CarNil Γ τ (d : Exp Γ τ) :
+    ValueP d →
+    Car d Nil ---> d
+  | ST_CarCons Γ τ (d x : Exp Γ τ) (xs : Exp Γ (TyList τ)) :
+    ValueP d →
+    ValueP x →
+    ValueP xs →
+    Car d (Cons x xs) ---> x
+
+  | ST_Cdr1 Γ τ (l l' : Exp Γ (TyList τ)) :
+    l ---> l' →
+    Cdr l ---> Cdr l'
+  | ST_CdrNil Γ τ :
+    Cdr (Nil (Γ:=Γ) (τ:=τ)) ---> Nil
+  | ST_CdrCons Γ τ (x : Exp Γ τ) (xs : Exp Γ (TyList τ)) :
+    ValueP x →
+    ValueP xs →
+    Cdr (Cons x xs) ---> xs
+
+  | ST_AppHost Γ dom cod (f : HostExp (dom ⟶ cod)) (v : Exp Γ dom) :
+    ∀ H : ValueP v,
+    APP (HostedFun f) v ---> CallHost f v H
+
+  | ST_AppAbs Γ dom cod (e : Exp (dom :: Γ) cod) (v : Exp Γ dom) :
+    ValueP v →
+    APP (LAM e) v ---> SubExp {|| v ||} e
+
+  | ST_App1 Γ dom cod (e1 : Exp Γ (dom ⟶ cod)) e1' (e2 : Exp Γ dom) :
+    e1 ---> e1' →
+    APP e1 e2 ---> APP e1' e2
+
+  | ST_App2 Γ dom cod (v1 : Exp Γ (dom ⟶ cod)) (e2 : Exp Γ dom) e2' :
+    ValueP v1 →
+    e2 ---> e2' →
+    APP v1 e2 ---> APP v1 e2'
+
+  where " t '--->' t' " := (Step t t').
+
+Derive Signature for Step.
+
+End Step.
+
+Notation " t '--->' t' " := (Step t t') (at level 40).
+
+Class HostLang (A : Type) : Type := {
+  has_host_exprs_sem :> HostExprsSem A;
+
+
+  CallHost_sound {Γ dom cod} (f : HostExp (dom ⟶ cod))
+                 (v : Exp Γ dom) (H : ValueP v) se :
+    HostExpSem f (SemExp v se) = SemExp (CallHost f v H) se;
+
+  CallHost_irr {Γ dom cod} (f : HostExp (dom ⟶ cod))
+               (v : Exp Γ dom) (H : ValueP v) :
+    ¬ (CallHost f v H = APP (HostedFun f) v);
+
+  CallHost_preserves_renaming {Γ Γ' dom cod} (f : HostExp (dom ⟶ cod))
+               (v : Exp Γ dom) (H : ValueP v) (σ : Ren Γ' Γ) :
+    APP (HostedFun f) (RenExp σ v) ---> RenExp σ (CallHost f v H);
+
+  CallHost_preserves_substitution {Γ Γ' dom cod} (f : HostExp (dom ⟶ cod))
+               (v : Exp Γ dom) (H : ValueP v) (σ : Sub Γ' Γ) :
+    APP (HostedFun f) (SubExp σ v) ---> SubExp σ (CallHost f v H);
+
+
+  Reduce_sound {Γ τ} (h : HostExp τ) se :
+    HostExpSem h = SemExp (projT1 (Reduce (Γ:=Γ) h)) se;
+
+  Reduce_irr {Γ τ} (h : HostExp τ) :
+    ¬ (projT1 (Reduce (Γ:=Γ) h) = HostedExp h);
+
+  Reduce_preserves_renaming {Γ Γ' τ} (h : HostExp τ) (σ : Ren Γ Γ') :
+    RenExp σ (HostedExp h) ---> RenExp σ (projT1 (Reduce h));
+
+  Reduce_preserves_substitution {Γ Γ' τ} (h : HostExp τ) (σ : Sub Γ Γ') :
+    SubExp σ (HostedExp h) ---> SubExp σ (projT1 (Reduce h));
+}.
+
+Section Sound.
+
+Context {A : Type}.
+Context `{L : HostLang A}.
+
+Theorem Step_sound {Γ τ} (e : Exp Γ τ) v :
+  e ---> v → SemExp e = SemExp v.
+Proof.
+  intros.
+  dependent induction H; simpl; auto;
+  extensionality se;
+  try now rewrite IHStep.
+  - now erewrite Reduce_sound; eauto.
+  - now apply CallHost_sound.
+  - rewrite <- SemExp_SubSem.
+    f_equal; simpl.
+    simp SubSem.
+    now rewrite SubSem_idSub.
+Qed.
+
+Lemma If_loop_true {Γ τ} b {x : Exp Γ τ} {y : Exp Γ τ} :
+  ¬ (If b x y = x).
+Proof.
+  induction x; intro; inv H.
+  now eapply IHx2; eauto.
+Qed.
+
+Lemma If_loop_false {Γ τ} b {x : Exp Γ τ} {y : Exp Γ τ} :
+  ¬ (If b x y = y).
+Proof.
+  induction y; intro; inv H.
+  now eapply IHy3; eauto.
+Qed.
+
+Lemma Seq_loop {Γ τ ty} {x : Exp Γ ty} {y : Exp Γ τ} :
+  ¬ (Seq x y = y).
+Proof.
+  induction y; intro; inv H.
+  now eapply IHy2; eauto.
+Qed.
+
+Lemma App_Lam_loop {Γ τ ty} {v : Exp Γ ty} {e : Exp (ty :: Γ) τ} :
+  ¬ (SubExp {||v||} e = APP (LAM e) v).
+Proof.
+  dependent induction e; repeat intro; inv H.
+  - dependent induction v0; simp consSub in *.
+    + simp SubVar in H1.
+      now induction v; inv H1; intuition.
+    + simp SubVar in H1.
+      rewrite SubVar_idSub in H1.
+      now induction v0; inv H1; intuition.
+  - admit.
+Admitted.
+
+(* A term never reduces to itself. *)
+#[export]
+Program Instance Step_Irreflexive {Γ τ} :
+  Irreflexive (Step (Γ:=Γ) (τ:=τ)).
+Next Obligation.
+  dependent induction x; try solve [ now inv H ].
+  - inv H.
+    + now apply Reduce_irr in H4.
+  - inv H.
+    + now eapply If_loop_true; eauto.
+    + now eapply If_loop_false; eauto.
+    + now firstorder.
+  - inv H.
+    now eapply Seq_loop; eauto.
+  - inv H.
+    + now eapply CallHost_irr; eauto.
+    + now eapply App_Lam_loop; eauto.
+    + now eapply IHx1; eauto.
+    + now eapply IHx2; eauto.
+Qed.
+
+#[export]
+Program Instance RenExp_Step {Γ Γ' τ} (σ : Ren Γ' Γ) :
+  Proper (Step (Γ:=Γ) (τ:=τ) ==> Step) (RenExp σ).
+Next Obligation.
+  intros.
+  induction H; simpl;
+  try solve [ now constructor; intuition idtac
+            | now constructor; intuition; apply RenExp_ValueP ].
+  - now apply Reduce_preserves_renaming.
+  - now apply CallHost_preserves_renaming.
+  - rewrite <- SubExp_ScR.
+    simp ScR.
+    rewrite <- RcS_idSub.
+    pose proof (SubExp_RcS (Keep σ) (Push (RenExp σ v) idSub) e).
+    simp RcS in H.
+    rewrite H.
+    constructor.
+    now apply RenExp_ValueP.
+Qed.
+
+#[export]
+Program Instance SubExp_Step {Γ Γ' τ} (σ : Sub Γ' Γ) :
+  Proper (Step (Γ:=Γ) (τ:=τ) ==> Step) (SubExp σ).
+Next Obligation.
+  intros.
+  induction H; simpl;
+  try solve [ now constructor; intuition idtac
+            | now constructor; intuition; apply SubExp_ValueP ].
+  - now apply Reduce_preserves_substitution.
+  - now apply CallHost_preserves_substitution.
+  - rewrite <- SubExp_ScS.
+    simpl ScS.
+    rewrite ScS_idSub_left.
+    pose proof (SubExp_ScS (Keepₛ σ) (Push (SubExp σ v) idSub) e).
+    simpl in H.
+    simp SubVar in H.
+    unfold Dropₛ in H.
+    rewrite ScS_ScR in H.
+    rewrite RcS_skip1 in H.
+    rewrite ScS_idSub_right in H.
+    rewrite H.
+    constructor.
+    now apply SubExp_ValueP.
+Qed.
+
+Corollary Step_productive {Γ τ} {x x' : Exp Γ τ} : x ---> x' → x ≠ x'.
+Proof.
+  repeat intro; subst.
+  now eapply Step_Irreflexive; eauto.
+Qed.
+
+Import ListNotations.
+
+Theorem strong_progress {τ} (e : Exp [] τ) :
+  ValueP e + { e' | e ---> e' }.
+Proof.
+  dependent induction e; reduce.
+  - destruct τ;
+    right; now exists (projT1 (Reduce h)); constructor.
+  - now left; constructor.
+  - now left; constructor.
+  - now left; constructor.
+  - now left; constructor.
+  - now left; constructor.
+  - right.
+    destruct IHe1; reduce.
+    + inv v.
+      * now exists e2; constructor.
+      * now exists e3; constructor.
+    + reduce.
+      now exists (If x e2 e3); constructor.
+  - destruct IHe1; reduce.
+    + destruct IHe2; reduce.
+      * left.
+        now constructor.
+      * right; reduce.
+        now exists (Pair e1 x); constructor.
+    + destruct IHe2; reduce.
+      * right; reduce.
+        now exists (Pair x e2); constructor.
+      * right; reduce.
+        now exists (Pair x e2); constructor.
+  - destruct IHe; reduce.
+    + right.
+      inv v; reduce.
+      * now exists x; constructor.
+    + right; reduce.
+      now exists (Fst x); constructor.
+  - destruct IHe; reduce.
+    + right.
+      inv v.
+      * now exists y; constructor.
+    + right; reduce.
+      now exists (Snd x); constructor.
+  - now left; constructor.
+  - destruct IHe1.
+    + destruct IHe2.
+      * now left; constructor.
+      * right; reduce.
+        now exists (Cons e1 x); constructor.
+    + destruct IHe2.
+      * right; reduce.
+        now exists (Cons x e2); constructor.
+      * right; reduce.
+        now exists (Cons x0 e2); constructor.
+  - destruct IHe1.
+    + destruct IHe2.
+      * right.
+        inv v0.
+        ** now eexists; constructor.
+        ** now eexists; constructor.
+      * right; reduce.
+        now exists (Car e1 x); constructor.
+    + destruct IHe2.
+      * right; reduce.
+        now exists (Car x e2); constructor.
+      * right; reduce.
+        now exists (Car x0 e2); constructor.
+  - destruct IHe.
+    + right.
+      inv v; now eexists; constructor.
+    + right; reduce.
+      now exists (Cdr x); constructor.
+  - right.
+    now exists e2; constructor.
+  - now inversion v.
+  - left.
+    now constructor.
+  - right.
+    destruct IHe1.
+    + destruct IHe2.
+      * dependent elimination e1; inv v.
+        ** now exists (CallHost h1 e2 v0); constructor.
+        ** now eexists (SubExp {|| e2 ||} _); constructor.
+      * dependent elimination e1; inv v.
+        ** exists (APP (HostedFun h1) x); constructor; auto.
+           now constructor.
+        ** eexists (APP (LAM _) x); constructor; eauto.
+           now constructor.
+    + reduce.
+      destruct IHe2.
+      * exists (APP x e2).
+        now constructor.
+      * reduce.
+        exists (APP x e2).
+        now constructor.
+Qed.
+
+End Sound.
